concurrency/dry_machine.v
@@ -243,10 +243,8 @@ Module Concur.
           threadHalted' cnt.
     
     Definition threadHalted: forall {tid0 ms},
-                               containsThread ms tid0 -> Prop:= @threadHalted'.
-
-    Parameter init_core : G -> val -> list val -> option thread_pool.
-
+        containsThread ms tid0 -> Prop:= @threadHalted'.
+    
     Definition one_pos : pos := mkPos NPeano.Nat.lt_0_2.
 
     Definition compute_init_perm : G -> access_map := fun _ => empty_map. (*Needst to be filled*)
